Use %testDafnyForEachResolver in VSComp

Test/VSComp2010/Problem4-Queens.dfy
@@ -1,5 +1,4 @@
-// RUN: %dafny /compile:0 /deprecation:0 "%s" > "%t"
-// RUN: %diff "%s.expect" "%t"
+// RUN: %testDafnyForEachResolver "%s" -- --relax-definite-assignment
 
 // VSComp 2010, problem 4, N queens
 // Rustan Leino, 31 August 2010, updated 24 March 2011.
@@ -32,28 +31,27 @@
 // given N.  If 'success' returns as 'true', 'board' indicates a solution.  If 'success'
 // returns as 'false', no solution exists, as stated in the second postcondition.
 method Search(N: int) returns (success: bool, board: seq<int>)
-  requires 0 <= N;
+  requires 0 <= N
   ensures success ==>
               |board| == N &&
-              (forall p :: 0 <= p && p < N ==> IsConsistent(board, p));
+              forall p :: 0 <= p && p < N ==> IsConsistent(board, p)
   ensures !success ==>
-              (forall B: seq<int> ::
+              forall B: seq<int> ::
                   |B| == N && (forall i :: 0 <= i && i < N ==> 0 <= B[i] && B[i] < N)
                   ==>
-                  (exists p :: 0 <= p && p < N && !IsConsistent(B, p)));
+                  exists p :: 0 <= p && p < N && !IsConsistent(B, p)
 {
   success, board := SearchAux(N, []);
 }
 
 // Given a board, this function says whether or not the queen placed in column 'pos'
 // is consistent with the queens placed in columns to its left.
-function IsConsistent(board: seq<int>, pos: int): bool
-{
+predicate IsConsistent(board: seq<int>, pos: int) {
   0 <= pos && pos < |board| &&
-  (forall q :: 0 <= q && q < pos ==>
+  forall q :: 0 <= q && q < pos ==>
       board[q] != board[pos] &&
       board[q] - board[pos] != pos - q &&
-      board[pos] - board[q] != pos - q)
+      board[pos] - board[q] != pos - q
 }
 
 // Here comes the method where the real work is being done.  With an ultimate board size of 'N'
@@ -62,19 +60,19 @@ function IsConsistent(board: seq<int>, pos: int): bool
 // then 'newBoard' is a consistent placement of 'N' queens.  If 'success' returns as 'false',
 // then there is no way to extend 'boardSoFar' to get a solution for 'N' queens.
 method SearchAux(N: int, boardSoFar: seq<int>) returns (success: bool, newBoard: seq<int>)
-  requires 0 <= N && |boardSoFar| <= N;
+  requires 0 <= N && |boardSoFar| <= N
   // consistent so far:
-  requires (forall k :: 0 <= k && k < |boardSoFar| ==> IsConsistent(boardSoFar, k));
+  requires forall k :: 0 <= k && k < |boardSoFar| ==> IsConsistent(boardSoFar, k)
   ensures success ==>
               |newBoard| == N &&
-              (forall p :: 0 <= p && p < N ==> IsConsistent(newBoard, p));
+              forall p :: 0 <= p && p < N ==> IsConsistent(newBoard, p)
   ensures !success ==>
-              (forall B: seq<int> ::
+              forall B: seq<int> ::
                   |B| == N && (forall i :: 0 <= i && i < N ==> 0 <= B[i] && B[i] < N) &&
                   boardSoFar <= B
                   ==>
-                  (exists p :: 0 <= p && p < N && !IsConsistent(B, p)));
-  decreases N - |boardSoFar|;
+                  exists p :: 0 <= p && p < N && !IsConsistent(B, p)
+  decreases N - |boardSoFar|
 {
   var pos := |boardSoFar|;
   if (pos == N) {
@@ -85,8 +83,8 @@ method SearchAux(N: int, boardSoFar: seq<int>) returns (success: bool, newBoard:
     // Exhaustively try all possibilities for the new column, 'pos'.
     var n := 0;
     while (n < N)
-      invariant n <= N;
-      invariant (forall B: seq<int> ::
+      invariant n <= N
+      invariant forall B: seq<int> ::
                   // For any board 'B' with 'N' queens, each placed in an existing row
                   |B| == N && (forall i :: 0 <= i && i < N ==> 0 <= B[i] && B[i] < N) &&
                   // ... where 'B' is an extension of 'boardSoFar'
@@ -96,11 +94,11 @@ method SearchAux(N: int, boardSoFar: seq<int>) returns (success: bool, newBoard:
                   0 <= B[pos] && B[pos] < n
                   ==>
                   // ... the board 'B' is not entirely consistent
-                  (exists p :: 0 <= p && p < N && !IsConsistent(B, p)));
+                  exists p :: 0 <= p && p < N && !IsConsistent(B, p)
     {
       // Let's try to extend the board-so-far with a queen in column 'n':
       var candidateBoard := boardSoFar + [n];
-      if (IsConsistent(candidateBoard, pos)) {
+      if IsConsistent(candidateBoard, pos) {
         // The new queen is consistent.  Thus, 'candidateBoard' is consistent in column 'pos'.
         // The consistency of the queens in columns left of 'pos' follows from the
         // consistency of those queens in 'boardSoFar' and the fact that 'candidateBoard' is
@@ -113,7 +111,7 @@ method SearchAux(N: int, boardSoFar: seq<int>) returns (success: bool, newBoard:
         // Thus, we meet the precondition of 'SearchAux' on 'candidateBoard', so let's search
         // for a solution that extends 'candidateBoard'.
         var s, b := SearchAux(N, candidateBoard);
-        if (s) {
+        if s {
           // The recursive call to 'SearchAux' found consistent positions for all remaining columns
           newBoard := b;
           success := true;
@@ -124,11 +122,11 @@ method SearchAux(N: int, boardSoFar: seq<int>) returns (success: bool, newBoard:
       } else {
         // Since 'n' is not a consistent placement for a queen in column 'pos', there is also
         // no extension of 'candidateBoard' that would make the entire board consistent.
-        assert (forall B: seq<int> ::
+        assert forall B: seq<int> ::
                   |B| == N && (forall i :: 0 <= i && i < N ==> 0 <= B[i] && B[i] < N) &&
                   candidateBoard <= B
                   ==>
-                  !IsConsistent(B, pos));
+                  !IsConsistent(B, pos);
       }
       n := n + 1;
     }
@@ -137,8 +135,7 @@ method SearchAux(N: int, boardSoFar: seq<int>) returns (success: bool, newBoard:
   }
 }
 
-method Main()
-{
+method Main() {
   var s, b := Search(2);
   print "N=2 returns ", s, "\n";
   s, b := Search(4);
@@ -146,11 +143,8 @@ method Main()
   PrintSeq(b);
 }
 
-method PrintSeq(b: seq<int>)
-{
-  var i := 0;
-  while (i < |b|) {
+method PrintSeq(b: seq<int>) {
+  for i := 0 to |b| {
     print "  ", b[i], "\n";
-    i := i + 1;
   }
 }
